Make progress on get_item_ok
Dealt with readers by having specs specifically say nobody is reading
the particular block. This is an "invariant" in the sense of being in
the pre/post of every method, but from the system's perspective it
can't be in Inv since the LockedDisk will have to yield after starting
a read.

We would like to say nobody is reading any RecArray address (which is a
simpler invariant), but we can only guarantee this for locked items.

Much of this proof is list manipulation. Proved some of these already,
so they do not represent most of the remaining work.

src/ConcurrentRecArray.v
@@ -10,6 +10,7 @@ Require Import Linearizable2.
 Require Import Rec.
 Require Import Arith.
 Require Import GenericArray.
+Require Import Omega.
 Import ConcurrentDisk.
 
 Import EqNotations.
@@ -101,6 +102,12 @@ Module RecArray (Params:RecArrayParams).
     inversion H0.
   Qed.
 
+  Corollary items_per_valu_gt_0 : 0 < items_per_valu.
+  Proof.
+    pose proof items_per_valu_not_0.
+    omega.
+  Qed.
+
   (* array_item_pairs *)
   Definition rep_blocks (vs : list block) : @pred addr _ (const valu) :=
     ([[ length vs = RALen ]] *
@@ -147,8 +154,6 @@ Module RecArray (Params:RecArrayParams).
       rewrite IHl.
       rewrite <- app_assoc; auto.
     Qed.
-
-    Require Import Omega.
 
     Ltac unify_in :=
       try lazymatch goal with
@@ -343,13 +348,16 @@ Module RecArray (Params:RecArrayParams).
     rep_blocks (nest_list vs items_per_valu).
 
   Definition rep_blocks' vs_nested (vd: Disk) :=
-    length vs_nested = RALen /\
     forall (a:addr), ($ RAStart <= a)%word ->
          (a < $ (RAStart + RALen))%word ->
+         (* TODO: selecting a is wrong here; this rep should really
+         quantify over a nat offset *)
          vd a = Some (block_valu (sel vs_nested a block0)).
 
-  Definition rep_items' (vs: list item) :=
-    rep_blocks' (nest_list vs items_per_valu).
+  Definition rep_items' (vs: list item) vd :=
+    rep_blocks' (nest_list vs items_per_valu) vd /\
+    length vs = RALen * items_per_valu /\
+    Forall Rec.well_formed vs.
 
   Module Type RecArrayVars (SemVars:SemanticsVars).
     Import SemVars.
@@ -474,7 +482,7 @@ Module RecArray (Params:RecArrayParams).
                let b := valu_block v in
                rx (get_block_offset b off).
 
-    Hint Resolve items_per_valu_not_0.
+    Hint Resolve items_per_valu_not_0 items_per_valu_gt_0.
 
     Lemma ra_end_goodSize : goodSize addrlen (RAStart + RALen).
     Proof.
@@ -505,11 +513,18 @@ Module RecArray (Params:RecArrayParams).
       rewrite wordToNat_natToWord_idempotent'; auto.
     Qed.
 
-    Require Import Omega.
-
     Hint Resolve ra_end_goodSize.
 
     Hint Extern 5 (_ <= _) => omega.
+
+    Lemma valid_block_offset : forall i,
+        i < RALen * items_per_valu ->
+        i / items_per_valu < RALen.
+    Proof.
+      intros.
+      apply Nat.div_lt_upper_bound; auto.
+      rewrite mult_comm; auto.
+    Qed.
 
     Lemma block_idx_valid : forall i,
         i < RALen * items_per_valu ->
@@ -518,14 +533,113 @@ Module RecArray (Params:RecArrayParams).
          bidx < $ (RAStart + RALen))%word.
     Proof.
       unfold block_idx; cbn; intros.
-      assert (i / items_per_valu < RALen).
-      apply Nat.div_lt_upper_bound; auto.
-      rewrite mult_comm; auto.
+      apply valid_block_offset in H.
       split.
       - apply wle_le''; auto.
-        eapply goodSize_trans with (n2 := RAStart + RALen); auto.
+        eapply goodSize_trans with (RAStart + RALen); auto.
       - apply wlt_lt''; auto.
     Qed.
+
+    Lemma block_idx_goodSize : forall i,
+        i < RALen * items_per_valu ->
+        # (@natToWord addrlen (block_idx i)) = block_idx i.
+    Proof.
+      unfold block_idx; intros.
+      apply valid_block_offset in H.
+      rewrite wordToNat_natToWord_idempotent'; auto.
+      eapply goodSize_trans with (RAStart + RALen); auto.
+    Qed.
+
+    Definition not_reading (vd: DISK) a :=
+      forall v, vd a = Some v -> snd v = None.
+
+    Definition not_reading' (vd: DISK) a :=
+      forall v, hide_readers vd a = Some v ->
+           vd a = Some (v, None).
+
+    Theorem not_reading_hide (vd: DISK) a :
+      not_reading vd a <->
+      not_reading' vd a.
+    Proof.
+      unfold not_reading, not_reading', hide_readers.
+      split; intros.
+      - destruct matches in *; try congruence.
+        inv_opt.
+        pose proof (H _ H1).
+        cbn in *; subst; auto.
+      - destruct v.
+        rewrite H0 in *.
+        specialize (H w); intuition idtac.
+        inv_opt; auto.
+    Qed.
+
+    Theorem not_reading_pair (vd: DISK) a :
+      not_reading vd a <->
+      forall v r, vd a = Some (v, r) -> r = None.
+    Proof.
+      unfold not_reading; split; intros.
+      apply (H _ H0).
+      destruct v; eauto.
+    Qed.
+
+    Theorem subslice_hom_selN : forall A (l: list (list A)) k i def,
+        i < length l ->
+        Forall (fun l => length l = k) l ->
+        skipn (i * k) (firstn (i * k + k) (concat l)) =
+        selN l i def.
+    Proof.
+      intros.
+      generalize dependent i.
+      induction l; cbn; intros.
+      inversion H.
+
+      inversion H0; subst; intuition.
+      destruct i; cbn.
+      replace (length a) with (length a + 0) by omega.
+      rewrite firstn_app_r; cbn.
+      rewrite app_nil_r; auto.
+      rewrite <- plus_assoc.
+      rewrite firstn_app_r; cbn.
+      rewrite skipn_app_r; cbn.
+      eauto.
+    Qed.
+
+    Theorem selN_nested : forall A (l: list A) k m i def,
+        0 < k ->
+        i < m ->
+        length l = m * k ->
+        selN (nest_list l k) i def =
+        skipn (i*k) (firstn (i*k+k) l).
+    Proof.
+      intros.
+      assert (0 < length l).
+      destruct m; cbn in *; try omega.
+      pose proof (le_0_n (m * k)).
+      omega.
+      rewrite <- nest_list_concat with (k := k) (l := l) at 2.
+      erewrite subslice_hom_selN; eauto.
+      erewrite length_nest_list_exact; eauto; try omega.
+      eapply nest_list_length; eauto.
+    Qed.
+
+    Theorem selN_subslice : forall A (l: list A) n m i def,
+        n + i < m ->
+        selN (skipn n (firstn m l)) i def =
+        selN l (n+i) def.
+    Proof.
+      intros.
+      rewrite skipn_selN.
+      rewrite selN_firstn; auto.
+    Qed.
+
+    Lemma off_idx_bound : forall i,
+        off_idx i < items_per_valu.
+    Proof.
+      intros.
+      apply Nat.mod_upper_bound; auto.
+    Qed.
+
+    Hint Resolve off_idx_bound.
 
     Polymorphic Theorem locked_get_item_ok : forall i,
         stateS TID: tid |-
@@ -534,11 +648,13 @@ Module RecArray (Params:RecArrayParams).
              Inv m s d /\
              Locks.get (get GLocks s) ($ (block_idx i)) = Owned tid /\
              i < RALen * items_per_valu /\
+             not_reading (view Latest (get GDisk s)) ($ (block_idx i)) /\
              R tid s0 s
          | POST d' m' s0' s' r:
                Inv m' s' d' /\
                locks_increasing tid s s' /\
                r = selN (get Items s') i item0 /\
+               not_reading (view Latest (get GDisk s')) ($ (block_idx i)) /\
                R tid s0' s'
         }} locked_get_item i.
     Proof.
@@ -546,16 +662,31 @@ Module RecArray (Params:RecArrayParams).
       step pre simplify with try solve [ finish ].
       intuition.
       unfold recarrayI, rep_items', rep_blocks' in *; intuition.
-      specialize (H11 ($ (block_idx i))).
+      specialize (H9 ($ (block_idx i))).
       let H := fresh in
       pose proof (@block_idx_valid i) as H; cbn in H.
       intuition idtac.
-      (* need a way for all specs to say we're not reading our locked
-      block, but we can't actually put that in the invariant
+      apply not_reading_hide in H3; unfold not_reading' in H3.
+      eauto.
 
-       interesting point: concretely, what breaks down if the
-       invariant says nobody is reading anything? the LockedDisk read
-       spec certainly won't be provable, but what axiom isn't true? *)
+      step pre simplify with try solve [ finish ].
+      unfold get_block_offset.
+      rewrite block_valu_id.
+      unfold recarrayI, rep_items', rep_blocks' in *; intuition.
+
+      unfold sel.
+      rewrite block_idx_goodSize by auto.
+
+      erewrite selN_nested; try omega.
+      rewrite selN_subslice; try omega.
+      (* TODO: not actually true, due to bug in rep; RAStart shouldn't
+      be part of these offsets *)
+      admit.
+
+      pose proof (off_idx_bound i); omega.
+      auto.
+      2: eauto.
+      (* this is wrong again due to the incorrect rep; it should be i, not block_idx i *)
     Abort.
 
   End RecArray.
